---
layout: math_post
title: Prologue - Problem 1
date: 2022-08-02
categories: article spivak calculus prologue
head_title: Prologue - Problem 1
meta_description: Spivak Calculus Prologue Problem 1
meta_keywords: spivak,calculus,prologue,solutions
---

We have to prove the following assertions:

<p>
<strong>(i)</strong> If $ax = a$ for some number $a\ne0$, then $x = 1$.

\[
  \begin{align*}
    ax &= a \\
    aa^{-1}x &= aa^{-1} && \text{| P8} \\
    x &= 1 && \text{| P7}
  \end{align*}   
\]
</p>

<p>
<strong>(ii)</strong> $x^2 - y^2 = (x - y)(x + y)$.

\[
  \begin{align*}
    (x - y)(x + y) &= x^2 + xy - yx - y^2 && \text{| P9} \\
                   &= x^2 + xy - xy - y^2 && \text{| P8} \\
                   &= x^2 - y^2 && \text{| P3}
  \end{align*}   
\]
</p>

<p>
<strong>(iii)</strong> If $x^2 = y^2$, then $x = y$ or $x = -y$.

\[
  \begin{align*}
    x^2 &= y^2 \\
    x^2 - y^2 &= 0 && \text{| P3} \\
    (x + y)(x - y) &= 0 && \text{| see (ii)}
  \end{align*}   
\]

Now we have 2 options. First:

\[
  \begin{align*}
      (x + y)(x - y)(x - y)^{-1} &= 0(x - y)^{-1} \\
      (x + y) &= 0 && \text{| P7 and 0a = 0} \\
      x &= -y && \text{| P3}
  \end{align*}   
\]

Second:

\[
  \begin{align*}
      (x + y)(x - y)(x + y)^{-1} &= 0(x + y)^{-1} \\
      (x - y) &= 0 && \text{| P8, P7 and 0a = 0} \\
      x &= y && \text{| P3}
  \end{align*}   
\]
</p>

<p>
<strong>(iv)</strong> $x^3 - y^3 = (x - y)(x^2 + xy + y^2)$. (From here on I will only occasionally reference the central properties.)

\[
  \begin{align*}
      (x - y)(x^2 + xy + y^2) &= x^3 + x^2y + xy^2 - x^2y - xy^2 - y^3 \\
                              &= x^3 - y^3 
  \end{align*}   
\]
</p>

<p>
<strong>(v)</strong> $x^n - y^n = (x - y)(x^{n - 1} + x^{n - 2}y + ... + xy^{n - 2} + y^{n - 1})$. This one is a bit tricky, because we have to be aware that the right-hand side of the equation is generated by the following sum:

\[
  (x - y)\sum_{j = 0}^{n - 1}x^jy^{n - 1 - j}
\]

Let's take $n = 3$ as an known example:

\[
  \sum_{j = 0}^{2}x^jy^{2 - j} = y^2 + xy + x^2 \text{ | } x^0 = 1
\]

This is equivalent to what we have in (iv). With that we can now rewrite the problem to:

\[
  \begin{align*}
      (x^n - y^n) &= (x - y)\sum_{j = 0}^{n - 1}x^jy^{n - 1 - j} \\
                  &= \sum_{j = 0}^{n - 1}x^{j + 1}y^{n - 1 - j} - \sum_{k = 0}^{n - 1}x^ky^{n - k} \\
                  &= x^n + \sum_{j = 0}^{n - 2}x^{j + 1}y^{n - 1 - j} - y^n - \sum_{k = 1}^{n - 1}x^ky^{n - k} \\
                  &= x^n - y^n + (\sum_{j = 0}^{n - 2}x^{j + 1}y^{n - 1 - j} - \sum_{k = 1}^{n - 1}x^ky^{n - k})
  \end{align*}
\]

We now have to show that $(\sum_{j = 0}^{n - 2}x^{j + 1}y^{n - 1 - j} - \sum_{k = 1}^{n - 1}x^ky^{n - k}) = 0$.

\[
  \begin{align*}
      \sum_{j = 0}^{n - 2}x^{j + 1}y^{n - 1 - j} - \sum_{k = 1}^{n - 1}x^ky^{n - k} &= 0\\
      \sum_{j = 0}^{n - 2}x^{j + 1}y^{n - 1 - j} &= \sum_{k = 1}^{n - 1}x^ky^{n - k} && \text{| } k - 1 = j \\
      &= \sum_{j = 1 - 1}^{n - 1 - 1}x^{j + 1}y^{n - (j + 1)}\\
      &= \sum_{j = 0}^{n - 2}x^{j + 1}y^{n - 1 - j}
  \end{align*}
\]
</p>

<p>
<strong>(vi)</strong> $x^3 + y^3 = (x + y)(x^2 - xy + y^2)$.

Replacing $y$ with $-y$ produces:

\[
 x^3 + (-y)^3 = (x - y)(x^2 + xy + y^2)
\]

That is identical to (iv).
</p>